SATsolver/Experiment/DPLL/Theorem.lean
@@ -1,7 +1,7 @@
 import SATsolver.Experiment.DPLL.impl
 
-theorem internal_final_state{f: Formula}{v : Variables}{vz : v ≠ 0}{wf : f.wf ∧ v.wf f}{b : Bool}{t t' : Trail}{twf : t.wf ∧ ∀ n ∈ t.names, n ∈ f.names}:
-  internal t f v vz wf twf = (b, t') → t' ⊨ f ∨ b = false := by
+theorem internal_final_state{f: Formula}{v : Variables}{vz : v ≠ 0}{wf : f.wf ∧ v.wf f}{b : Bool}{t t' : Trail}{twf : t.wf ∧ ∀ n ∈ t.names, n ∈ f.names}{com : Completenes.inv t f}:
+  internal t f v vz wf twf com = (b, t') → t' ⊨ f ∨ b = false := by
   unfold internal
   split
   case isTrue hsat =>
@@ -58,6 +58,132 @@ DPLL f  v wf = (b, t) → t ⊨ f ∨ b = false := by
     simp
     exact internal_final_state
 
+theorem internal_all_deduced_if_con{f: Formula}{v : Variables}{vz : v ≠ 0}{wf : f.wf ∧ v.wf f}{b : Bool}{t t' : Trail}{twf : t.wf ∧ ∀ n ∈ t.names, n ∈ f.names}{com : Completenes.inv t f}:
+  internal t f v vz wf twf com = (b, t') → b = false → (t' ⊭ f ∧  ∀ a ∈ t', a.deducedP) := by
+  unfold internal
+  split
+  case isTrue =>
+    simp
+    intro btrue heq bfalse
+    simp[btrue] at bfalse
+  case isFalse hsat =>
+    split
+    case isTrue hcon =>
+      split
+      case isTrue hexi => exact internal_all_deduced_if_con
+      case isFalse hexi =>
+        simp[ALit.decidedP_iff_decidedB, ←ALit.ded_iff_not_dec] at hexi
+        intro heq bfalse
+        simp at heq
+        simp[←heq.2]
+        constructor
+        case left => simpa using hcon
+        case right => exact hexi
+    case isFalse hcon =>
+      simp
+      split
+      case isTrue hunit =>
+        exact internal_all_deduced_if_con
+      case isFalse hunit =>
+        exact internal_all_deduced_if_con
+  termination_by distance t v vz
+  decreasing_by
+    have : t.length < v := by
+      rename ¬decide (t⊨f) = true => sat
+      rename ¬decide (t⊭f) = true => con
+      simp at sat con
+      have := Trail.ud_vars twf.1 wf.1 wf.2 twf.2 (Formula.nSatCon_ud sat con)
+      simp[Trail.names] at this
+      exact this
+    exact distance_dec this
+    have : t.length < v := by
+      rename ¬decide (t⊨f) = true => sat
+      rename ¬decide (t⊭f) = true => con
+      simp at sat con
+      have := Trail.ud_vars twf.1 wf.1 wf.2 twf.2 (Formula.nSatCon_ud sat con)
+      simp[Trail.names] at this
+      exact this
+    exact distance_prop this
+    have : t.length ≤ v := Trail.mem_vwf twf.1 twf.2 wf.2
+    exact distance_bc this
+
+theorem internal_com_preserved {f: Formula}{v : Variables}{vz : v ≠ 0}{wf : f.wf ∧ v.wf f}{b : Bool}{t t' : Trail}{twf : t.wf ∧ ∀ n ∈ t.names, n ∈ f.names}{com : Completenes.inv t f}:
+  internal t f v vz wf twf com = (b, t') → Completenes.inv t' f := by
+  unfold internal
+  split
+  case isTrue hsat =>
+    intro heq
+    simp at heq
+    rw[←heq.2]
+    exact com
+  case isFalse hsat =>
+    split
+    case isTrue hcon =>
+      split
+      case isTrue exdec=>
+        intro h
+        simp at h
+        exact internal_com_preserved h
+      case isFalse exdec =>
+        intro heq
+        simp at heq
+        rw[←heq.2]
+        exact com
+    case isFalse hcon =>
+      simp
+      split
+      case isTrue exuni =>
+        exact internal_com_preserved
+      case isFalse exuni =>
+        exact internal_com_preserved
+  termination_by distance t v vz
+  decreasing_by
+    have : t.length < v := by
+      rename ¬decide (t⊨f) = true => sat
+      rename ¬decide (t⊭f) = true => con
+      simp at sat con
+      have := Trail.ud_vars twf.1 wf.1 wf.2 twf.2 (Formula.nSatCon_ud sat con)
+      simp[Trail.names] at this
+      exact this
+    exact distance_dec this
+    have : t.length < v := by
+      rename ¬decide (t⊨f) = true => sat
+      rename ¬decide (t⊭f) = true => con
+      simp at sat con
+      have := Trail.ud_vars twf.1 wf.1 wf.2 twf.2 (Formula.nSatCon_ud sat con)
+      simp[Trail.names] at this
+      exact this
+    exact distance_prop this
+    have : t.length ≤ v := Trail.mem_vwf twf.1 twf.2 wf.2
+    exact distance_bc this
+
+theorem DPLL.com_preserved {f : Formula}{v : Variables}{wf : f.wf ∧ v.wf f}{b : Bool}{t : Trail} :
+  DPLL f v wf = (b, t) → Completenes.inv t f := by
+  simp[DPLL]
+  cases f
+  case nil =>
+    simp
+    intro btrue heq
+    simp[heq, Completenes.inv]
+  case cons c cs =>
+    simp
+    intro h
+    exact internal_com_preserved h
+
+
+theorem DPLL.all_deduced_if_con {f : Formula}{v : Variables} {wf : f.wf ∧ v.wf f}{b : Bool}{t : Trail} :
+  DPLL f v wf = (b, t) → b = false → t ⊭ f ∧ ∀ a ∈ t, a.deducedP := by
+  simp[DPLL]
+  cases f
+  case nil =>
+    simp
+    intro btrue hnil bfalse
+    simp[btrue] at bfalse
+  case cons x xs =>
+    simp
+    intro heq bfalse
+    exact internal_all_deduced_if_con heq bfalse
+
 
 theorem DPLL.soundness {f : Formula}{v : Variables}{wf : f.wf ∧ v.wf f}{b : Bool}{t : Trail} :
   DPLL f  v wf = (b, t) → b = true → ∃ (t : Trail), t ⊨ f := by
@@ -66,8 +192,18 @@ theorem DPLL.soundness {f : Formula}{v : Variables}{wf : f.wf ∧ v.wf f}{b : Bo
   simp[bh] at this
   exists t
 
-theorem internal_final_false{f: Formula}{v : Variables}{vz : v ≠ 0}{wf : f.wf ∧ v.wf f}{t t' : Trail}{twf : t.wf ∧ ∀ n ∈ t.names, n ∈ f.names}:
-  internal t f v vz wf twf = (false, t') → ¬ (∃ (t : Trail), t ⊨ f) := by
+theorem DPLL.final_false{f: Formula}{v : Variables}{vz : v ≠ 0}{wf : f.wf ∧ v.wf f}{t t' : Trail}{twf : t.wf ∧ ∀ n ∈ t.names, n ∈ f.names}:
+  DPLL f v wf = (b, t) → b = false → ¬ (∃ (t : Trail), t.wf ∧ t ⊨ f) := by
+  intro heq bfalse
+  have state := DPLL.all_deduced_if_con heq bfalse
+  have com := DPLL.com_preserved heq
+  have := Completenes.inv_completeness twf.1 com state.2
+  simp at this ⊢
+  intro x xwf
+  have nohead := Completenes.from_con state.1
+  simp at nohead
+
+
   intro h
   unfold internal at h
   split at h
